experimental/ni_coq/vfiles/PossibilisticNI.v
@@ -1,0 +1,86 @@
+Require Import Coq.Lists.List.
+Import ListNotations.
+From OakIFC Require Import
+    Parameters
+    RuntimeModel
+    EvAugSemantics
+    Events
+    LowEquivalences.
+
+(*
+This is the top-level candidate security condition. This is a
+"possibilistic security condition". A possibilistic security condition
+says that two executions look the same from the perspective of an observer
+if all _possible behaviors_ look the same if they begin from initial states
+that look the same to the observer.
+In other words there is some way to reach an execution trace
+that looks the same beginning from the other state.
+
+Trapeze uses a possibilistic definition of security:
+https://pdfs.semanticscholar.org/809b/f2702a765b9e7dba4624a1dbc53af11579db.pdf
+See also:
+https://www.cs.cornell.edu/andru/papers/csfw03.pdf
+
+*)
+
+(* An alternative way of specifying security for
+   concurrent systems is observational determinism, which says
+   that for any two executions that begin from low-equivalent
+   initial states, all actual observed behaviors 
+   (by contrast to the possibly observed behaviors)
+   _always_ look the same.
+
+    This looks like:
+    forall s1 s2 t1 t2,
+        (s1 =L s2) /\
+        (step_multi s1) => t1 /\
+        (step_multi s2) => t2 ->
+            t1 =L t2.
+
+    An advantage of observational determinism over possibilistic
+    noninterference is that O.D. is preserved by refinement. This does
+    not matter in this context since we are not doing a refinement proof.
+    
+    O.D. also has requirements about data race freedom that are not
+    needed to prove a possibilistic security definition. (It may be
+    worth looking into whether or not the runtime actually satisfies
+    these data race freedom requirements later, though it does not
+    seem high priority).
+
+    ***
+    These two definitions also crucially require different
+    definitions of trace low-equivalence as discussed in Events.v
+    ***
+*)
+
+Definition conjecture_possibilistic_ni := forall ell s11 s21 s1n t1n,
+    (state_low_eq ell s11 s21) /\
+    (step_system_ev_multi s11 [] s1n t1n) ->
+    (exists s2n t2n,
+        (step_system_ev_multi s21 [] s2n t2n) /\
+        (trace_low_eq ell t1n t2n)).
+
+Theorem possibilistic_ni_1step: forall ell s11 s21 s12 t12,
+    (state_low_eq ell s11 s21) /\
+    (step_system_ev s11 [] s12 t12) ->
+    (exists s22 t22,
+        (step_system_ev s21 [] s22 t22) /\
+        (trace_low_eq ell t12 t22)).
+Admitted. (* NOTE: work in progress *)
+
+Theorem possibilistic_ni: conjecture_possibilistic_ni. Proof.
+unfold conjecture_possibilistic_ni.
+intros ell s11 s21 s1n t1n [H1 H2].
+remember ([]: trace) as emp eqn:R.
+induction H2 as [s11 t s12 t12 | s11 t s1' t1' s1n t1n]; rewrite R in *.
+- assert (E: (exists s22 t22,
+        (step_system_ev s21 [] s22 t22) /\
+        (trace_low_eq ell t12 t22))). {
+        apply (possibilistic_ni_1step ell s11 s21 s12 t12). split; assumption.
+}
+destruct E as [s22 E]. destruct E as [t22 [E1 E2]].
+exists s22, t22. split; try constructor; assumption.
+- (* no induction hypothesis *)(* induction on trace length instead  ? *)
+admit.
+(* NOTE: This is only admitted because it is work in progress *)
+Admitted.
